src/Monotonic.v
@@ -3,19 +3,23 @@ From Clairvoyance Require Import Core Approx.
 
 Create HintDb mon.
 
+Record less_defined_M {a} `{LessDefined a} (u v : M a) : Prop :=
+  { less_defined_M_def :
+    u {{ fun x n =>
+    v [[ fun y m => x `less_defined` y /\ m <= n ]] }} }.
+
 #[global] Instance LessDefined_M {a} `{LessDefined a} : LessDefined (M a) :=
-  fun u v =>
-  u {{ fun x n =>
-  v [[ fun y m => x `less_defined` y /\ m <= n ]] }}.
+  less_defined_M.
 
 #[global] Instance PreOrder_LessDefined_M {a} `{LessDefined a} `{!PreOrder (less_defined (a := a))}
   : PreOrder (less_defined (a := M a)).
 Proof.
   constructor.
-  - red. unfold less_defined, LessDefined_M, pessimistic, optimistic. firstorder.
-  - red. unfold less_defined, LessDefined_M, pessimistic, optimistic. firstorder.
-    edestruct H0 as (? & ? & ? & ? & ?); [ eassumption | ].
-    edestruct H1 as (? & ? & ? & ? & ?); [ eassumption | ].
+  - red. unfold less_defined, LessDefined_M. firstorder.
+  - red. unfold less_defined, LessDefined_M. intros * [HH1] [HH2]; constructor.
+    unfold pessimistic, optimistic in *. firstorder.
+    edestruct HH1 as (? & ? & ? & ? & ?); [ eassumption | ].
+    edestruct HH2 as (? & ? & ? & ? & ?); [ eassumption | ].
     eexists _, _; split; [ eassumption | split; etransitivity; eassumption ].
 Qed.
 
@@ -57,7 +61,7 @@ Qed.
 Lemma ret_mon {a} `{LessDefined a}
   : forall x y : a, x `less_defined` y -> ret x `less_defined` ret y.
 Proof.
-  intros. unfold less_defined, LessDefined_M.
+  intros. constructor.
   apply pessimistic_ret, optimistic_ret.
   split; auto.
 Qed.
@@ -71,7 +75,7 @@ Proof.
   | [ |- context [ less_defined (a := M ?a) ] ] =>
     let ld := eval unfold less_defined, LessDefined_M in (less_defined (a := M a)) in
     change (less_defined (a := M a)) with ld
-  end. intros * Hu * Hk.
+  end. intros * Hu * Hk. constructor.
   apply pessimistic_bind.
   relax; [ apply Hu | cbn; intros x n [x' [n' [Hu' [Hx' Hn'] ] ] ] ].
   relax; [ apply Hk; eassumption | cbn; intros * Hk' ].
@@ -84,33 +88,59 @@ Lemma force_mon {a} `{LessDefined a}
   : forall x y : T a, x `less_defined` y -> force x `less_defined` force y.
 Proof.
   intros ? ? []; cbn.
-  - hnf. contradiction.
+  - constructor. hnf. contradiction.
   - apply ret_mon; auto.
+Qed.
+
+Lemma forcing_mon {a b} `{LessDefined a, LessDefined b}
+  : forall x y : T a, x `less_defined` y ->
+    forall k h : a -> M b, (forall r s, r `less_defined` s -> k r `less_defined` h s) ->
+    forcing x k `less_defined` forcing y h.
+Proof.
+  intros; constructor; mforward idtac; intros ? ->.
+  inversion H1; subst. relax_apply H2. assumption.
 Qed.
 
 Lemma thunk_mon {a} `{LessDefined a} `{!PreOrder (less_defined (a := a))}
   : forall u v : M a, u `less_defined` v -> thunk u `less_defined` thunk v.
 Proof.
   unfold less_defined, LessDefined_M. intros u v Hu.
-  apply pessimistic_thunk.
+  constructor; apply pessimistic_thunk.
   - relax; [ apply Hu | cbn; intros * Hv ]. apply optimistic_thunk_go.
     relax; [ apply Hv | cbn; intros * [] ]. split; [ solve_approx idtac | auto ].
   - apply optimistic_skip. split; [ reflexivity | auto ].
 Qed.
 
+Lemma bot_mon {a} `{LessDefined a} (u : M a)
+  : (fun _ _ => False) `less_defined` u.
+Proof.
+  constructor; hnf; contradiction.
+Qed.
+
 Ltac solve_mon :=
   repeat
-    (eauto with mon;
+    (eassumption + reflexivity + eauto with mon;
     match goal with
     | [ H : less_defined _ _ |- _ ] =>
       let t := type of H in
       match eval hnf in t with
       | eq ?x ?y => change t with (eq x y) in H; subst x + subst y
       end
-    | [ |- less_defined _ _ ] => eassumption + reflexivity + constructor
-    | [ |- less_defined (match ?x with _ => _ end) (match ?x with _ => _ end) ] => let Ex := fresh "Ex" in destruct x eqn:Ex
-    | [ |- less_defined (ret _) (ret _) ] => apply ret_mon
-    | [ |- less_defined (bind _ _) (bind _ _) ] => apply bind_mon; [ | intros ? ? ? ]
-    | [ |- less_defined (force _) (force _) ] => apply force_mon
-    | [ |- less_defined (thunk _) (thunk _) ] => apply thunk_mon
+    end +
+    lazymatch goal with
+    | [ |- less_defined (a := M _) _ _ ] =>
+      match goal with
+      | [ |- less_defined (match ?x with _ => _ end) (match ?y with _ => _ end) ] =>
+        tryif constr_eq x y then let Ex := fresh "Ex" in destruct x eqn:Ex else
+        match goal with
+        | [ H : less_defined x y |- _ ] => inversion H
+        end
+      | [ |- less_defined (ret _) (ret _) ] => apply ret_mon
+      | [ |- less_defined (bind _ _) (bind _ _) ] => apply bind_mon; [ | intros ? ? ? ]
+      | [ |- less_defined (forcing _ _) (forcing _ _) ] => apply forcing_mon; [ | intros ? ? ? ]
+      | [ |- less_defined (force _) (force _) ] => apply force_mon
+      | [ |- less_defined (thunk _) (thunk _) ] => apply thunk_mon
+      | [ |- less_defined (fun _ _ => False) _ ] => apply bot_mon
+      end
+    | [ |- less_defined _ _ ] => constructor
     end).
